src/lib/kuiper/Kuiper.Epoch.fsti
@@ -4,18 +4,18 @@ module Kuiper.Epoch
 open Pulse
 open Kuiper.Kernel.Stream
 
-type epoch_t (s: stream_t) = erased nat
+type epoch_t = erased nat
 
-val epoch_live (#s: stream_t) (n:epoch_t s) : slprop
-val epoch_done (#s: stream_t) (n:epoch_t s) : slprop
+val epoch_live (s: stream_t) (n:epoch_t) : slprop
+val epoch_done (s: stream_t) (n:epoch_t) : slprop
 
 ghost
 fn get_epoch (s: stream_t) ()
-  returns e : epoch_t s
-  ensures epoch_live #s e
+  returns e : epoch_t
+  ensures epoch_live s e
 
 ghost
-fn done_lower (s: stream_t) (e f : epoch_t s)
-  preserves epoch_done #s e
+fn done_lower (s: stream_t) (e f : epoch_t)
+  preserves epoch_done s e
   requires pure (f <= e)
-  ensures  epoch_done #s f
+  ensures  epoch_done s f
