src/lib/kuiper/Kuiper.Kernel.fst
@@ -25,9 +25,9 @@ fn launch_kernel_full_sync
   get_epoch s ();
   launch_kernel_full k s;
   sync_stream s; 
-  redeem_pledge emp_inames (epoch_done #s _) (on gpu_loc full_post);
-  drop_ (epoch_done #s _);
-  drop_ (epoch_live #s _);
+  redeem_pledge emp_inames (epoch_done s _) (on gpu_loc full_post);
+  drop_ (epoch_done s _);
+  drop_ (epoch_live s _);
   destroy_stream s;
 }
 
